Remove DecType

src/classes/SMT_classes.v
@@ -17,41 +17,11 @@ From Stdlib Require Import Bool OrderedType.
     classes). *)
 
 
-(** Boolean equality to decidable equality *)
-Definition eqb_to_eq_dec :
-  forall T (eqb : T -> T -> bool) (eqb_spec : forall x y, eqb x y = true <-> x = y) (x y : T),
-    { x = y } + { x <> y }.
-  intros.
-  case_eq (eqb x y); intro.
-  left. apply eqb_spec; auto.
-  right. red. intro. apply eqb_spec in H0. rewrite H in H0. now contradict H0.
-  Defined.
-
-
 (** Types with a Boolean equality that reflects Leibniz equality *)
 Class EqbType T := {
  eqb : T -> T -> bool;
  eqb_spec : forall x y, eqb x y = true <-> x = y
 }.
-
-
-(** Types with a decidable equality *)
-Class DecType T := {
- eq_dec : forall x y : T, { x = y } + { x <> y }
-}.
-
-
-(** Types equipped with Boolean equality are decidable *)
-Section EqbToDecType.
-  Generalizable Variable T.
-  Context `{ET : EqbType T}.
-
-  Instance EqbToDecType : DecType T.
-  Proof.
-    destruct ET as [eqb0 Heqb0]. split.
-    apply (eqb_to_eq_dec _ eqb0); auto.
-  Defined.
-End EqbToDecType.
 
 
 (** Basic properties on types with Boolean equality *)
@@ -226,3 +196,272 @@ Register te_carrier as SMTCoq.classes.SMT_classes.te_carrier.
 Register te_compdec as SMTCoq.classes.SMT_classes.te_compdec.
 Register eqb_of_compdec as SMTCoq.classes.SMT_classes.eqb_of_compdec.
 Register CompDec as SMTCoq.classes.SMT_classes.CompDec.
+
+
+(* Compatibility of CompDec with standard type constructions *)
+
+Section list_EqbType.
+
+  Generalizable Variable A.
+  Context `{HA : EqbType A}.
+
+ Fixpoint eqb_list (xs ys:list A) : bool :=
+    match xs, ys with
+    | nil, nil => true
+    | x::xs, y::ys => eqb x y && eqb_list xs ys
+    | _, _ => false
+    end.
+
+  Lemma eqb_list_spec xs : forall ys, eqb_list xs ys = true <-> xs = ys.
+  Proof.
+    induction xs as [ |x xs IHxs]; intros [ |y ys]; split; simpl; intro H; auto; try discriminate.
+    - rewrite andb_true_iff in H. destruct H as [H1 H2].
+      rewrite eqb_spec in H1; subst.
+      now rewrite (IHxs ys) in H2; subst.
+    - injection H. intros -> ->. rewrite andb_true_iff; split.
+      + now rewrite eqb_spec.
+      + now rewrite IHxs.
+  Qed.
+
+  Global Instance list_eqbtype : EqbType (list A) :=
+    {| eqb := eqb_list;
+       eqb_spec := eqb_list_spec |}.
+
+End list_EqbType.
+
+
+Section list.
+
+  Generalizable Variable A.
+  Context `{HA : CompDec A}.
+
+
+  Fixpoint list_lt (xs ys : list A) : Prop :=
+    match xs, ys with
+    | nil, nil => False
+    | nil, _::_ => True
+    | _::_, nil => False
+    | x::xs, y::ys => (lt x y) \/ (eqb x y = true /\ list_lt xs ys)
+    end.
+
+
+  Definition list_compare : forall (x y : list A), Compare list_lt Logic.eq x y.
+  Proof.
+    induction x as [ |x xs IHxs]; intros [ |y ys]; simpl.
+    - now apply EQ.
+    - now apply LT.
+    - now apply GT.
+    - case_eq (compare x y); intros l H.
+      + apply LT. simpl. now left.
+      + case_eq (IHxs ys); intros l1 H1.
+        * apply LT. simpl. right. split; auto. now apply eqb_spec.
+        * apply EQ. now rewrite l, l1.
+        * apply GT. simpl. right. split; auto. now apply eqb_spec.
+      + apply GT. simpl. now left.
+  Defined.
+
+
+  Lemma list_lt_trans : forall (x y z : list A),
+      list_lt x y -> list_lt y z -> list_lt x z.
+  Proof.
+    induction x as [ |x xs IHxs]; intros [ |y ys] [ |z zs]; simpl; auto.
+    - inversion 1.
+    - intros [H1|[H1a H1b]] [H2|[H2a H2b]].
+      + left; eapply lt_trans; eauto.
+      + left. unfold is_true in H2a. rewrite eqb_spec in H2a. now subst z.
+      + left. unfold is_true in H1a. rewrite eqb_spec in H1a. now subst y.
+      + right. split.
+        * unfold is_true in H1a. rewrite eqb_spec in H1a. now subst y.
+        * eapply IHxs; eauto.
+  Qed.
+
+
+  Lemma list_lt_not_eq : forall (x y : list A), list_lt x y -> x <> y.
+  Proof.
+    induction x as [ |x xs IHxs]; intros [ |y ys]; simpl; auto.
+    - discriminate.
+    - intros [H1|[H1 H2]]; intros H; inversion H; subst.
+      + now apply (lt_not_eq _ _ H1).
+      + now apply (IHxs _ H2).
+  Qed.
+
+
+  Global Instance list_ord : OrdType (list A) :=
+    Build_OrdType _ _ list_lt_trans list_lt_not_eq.
+
+
+  Global Instance list_comp : Comparable (list A) := Build_Comparable _ _ list_compare.
+
+
+  Global Instance list_inh : Inhabited (list A) := Build_Inhabited _ nil.
+
+
+  Global Instance list_compdec : CompDec (list A) := {|
+    Ordered := list_ord;
+    Comp := list_comp;
+    Inh := list_inh
+  |}.
+
+End list.
+
+
+Section prod_EqbType.
+
+  Generalizable Variables A B.
+  Context `{HA : EqbType A} `{HB : EqbType B}.
+
+  Definition eqb_prod (x y:A * B) : bool :=
+    let (xa, xb) := x in
+    let (ya, yb) := y in
+    eqb xa ya && eqb xb yb.
+
+  Lemma eqb_prod_spec : forall x y, eqb_prod x y = true <-> x = y.
+  Proof.
+    intros [xa xb] [ya yb]; simpl; split; rewrite andb_true_iff.
+    - rewrite !eqb_spec. now intros [-> ->].
+    - intro H. rewrite !eqb_spec. now inversion H.
+  Qed.
+
+  Global Instance prod_eqbtype : EqbType (prod A B) :=
+    {| eqb := eqb_prod;
+       eqb_spec := eqb_prod_spec |}.
+
+End prod_EqbType.
+
+
+Section prod_OrdType.
+
+  Generalizable Variables A B.
+  Context `{HA : OrdType A} `{HB : OrdType B}.
+
+
+  Definition prod_lt (x y:A*B) : Prop :=
+    let (a1, b1) := x in
+    let (a2, b2) := y in
+    (lt a1 a2) \/ ((a1 = a2) /\ (lt b1 b2)).
+
+
+  Lemma prod_lt_trans : forall (x y z:A*B),
+      prod_lt x y -> prod_lt y z -> prod_lt x z.
+  Proof.
+    intros [a1 b1] [a2 b2] [a3 b3]; simpl.
+    intros [H1|[H1 H4]] [H2|[H2 H3]].
+    - left. eapply lt_trans; eauto.
+    - subst a3. now left.
+    - subst a2. now left.
+    - subst a2 a3. right. split; auto. eapply lt_trans; eauto.
+  Qed.
+
+
+  Lemma prod_lt_not_eq : forall (x y:A*B), prod_lt x y -> x <> y.
+  Proof.
+    intros [a1 b1] [a2 b2]; simpl.
+    intros [H1|[_ H1]] H3; inversion H3 as [[H4 H5]]; clear H3; subst a2 b2;
+      now apply (lt_not_eq _ _ H1).
+  Qed.
+
+
+  Global Instance prod_ord : OrdType (prod A B) :=
+    Build_OrdType _ _ prod_lt_trans prod_lt_not_eq.
+
+End prod_OrdType.
+
+
+Section prod.
+
+  Generalizable Variables A B.
+  Context `{HA : CompDec A} `{HB : CompDec B}.
+
+
+  Definition prod_compare : forall (x y:A*B), Compare lt Logic.eq x y.
+  Proof.
+    intros [a1 b1] [a2 b2].
+    case_eq (compare a1 a2); intros l H.
+    - apply LT. simpl. now left.
+    - case_eq (compare b1 b2); intros l1 H1.
+      + apply LT. simpl. now right.
+      + apply EQ. now subst.
+      + apply GT. simpl. now right.
+    - apply GT. simpl. now left.
+  Defined.
+
+
+  Global Instance prod_comp : Comparable (prod A B) := Build_Comparable _ _ prod_compare.
+
+
+  Global Instance prod_inh : Inhabited (prod A B) :=
+    Build_Inhabited _ (default_value, default_value).
+
+
+  Global Instance prod_compdec : CompDec (prod A B) := {|
+    Ordered := prod_ord;
+    Comp := prod_comp;
+    Inh := prod_inh
+  |}.
+
+End prod.
+
+
+Section option.
+
+  Generalizable Variable A.
+  Context `{HA : CompDec A}.
+
+
+  Definition option_lt (x y : option A) : Prop :=
+    match x, y with
+    | Some a, Some b => lt a b
+    | Some _, None => True
+    | None, Some _ => False
+    | None, None => False
+    end.
+
+
+  Lemma option_lt_trans : forall (x y z : option A),
+      option_lt x y -> option_lt y z -> option_lt x z.
+  Proof.
+    intros [a| ] [b| ] [c| ]; simpl; auto.
+    - apply lt_trans.
+    - intros _ [].
+  Qed.
+
+
+  Lemma option_lt_not_eq : forall (x y : option A), option_lt x y -> x <> y.
+  Proof.
+    intros [a| ] [b| ]; simpl; auto.
+    - intros H1 H2. inversion H2 as [H3]. revert H3. now apply lt_not_eq.
+    - discriminate.
+  Qed.
+
+
+  Global Instance option_ord : OrdType (option A) :=
+    Build_OrdType _ _ option_lt_trans option_lt_not_eq.
+
+
+  Definition option_compare : forall (x y : option A), Compare option_lt Logic.eq x y.
+  Proof.
+    intros [a| ] [b| ]; simpl.
+    - case_eq (compare a b); intros l H.
+      + now apply LT.
+      + apply EQ. now subst b.
+      + now apply GT.
+    - now apply LT.
+    - now apply GT.
+    - now apply EQ.
+  Defined.
+
+  Global Instance option_comp : Comparable (option A) := Build_Comparable _ _ option_compare.
+
+  Global Instance option_eqbtype : EqbType (option A) := Comparable2EqbType.
+
+
+  Global Instance option_inh : Inhabited (option A) := Build_Inhabited _ None.
+
+
+  Global Instance option_compdec : CompDec (option A) := {|
+    Ordered := option_ord;
+    Comp := option_comp;
+    Inh := option_inh
+  |}.
+
+End option.
